\begin{itemize}
	\item $ p \rightarrow q \equiv \lnot p \lor q$
	\item $ p \rightarrow q \equiv \lnot q \rightarrow \lnot p$
	\item $ p \lor q \equiv \lnot p \rightarrow q$
	\item $ p \land q \equiv \lnot (p \rightarrow \lnot q)$
	\item $ \lnot (p \rightarrow q) \equiv p \land \lnot q$
	\item $ (p \rightarrow q) \land (p \rightarrow r) \equiv p \rightarrow (q \land r)$
	\item $ (p \rightarrow q) \lor (p \rightarrow r) \equiv p \rightarrow (q \lor r)$
	\item $ (p \rightarrow r) \land (q \rightarrow r) \equiv (p \land q) \rightarrow r$
	\item $ (p \rightarrow r) \lor (q \rightarrow r) \equiv (p \lor q) \rightarrow r$
	\item $(p \land q) \lor (r \land s) \equiv (p \lor r) \land (p \lor s) \land (q \lor r) \land (q \lor s)$
\end{itemize}